aneris/examples/reliable_communication/lib/repdb/resources/log_resources.v
@@ -1,0 +1,44 @@
+From iris.algebra Require Import auth dfrac.
+From iris.algebra.lib Require Import mono_list.
+From iris.bi.lib Require Import fractional.
+From iris.proofmode Require Import tactics.
+From aneris.aneris_lang Require Import lang resources.
+
+
+(* ------------------------------------------------------------------------ *)
+ Section Log_Resources_definition.
+  Context `{!anerisG Mdl Σ}.
+  Context {Aty : Type}.
+  Notation A := (leibnizO Aty).
+  Context `{inG Σ (mono_listUR A)}.
+  (** Log resources. *)
+
+
+  (** ** Owned by global invariant of the system. *)
+  Definition own_log_auth (γ : gname) (q : Qp) (l : list A) : iProp Σ :=
+    own γ (●ML{ DfracOwn q } l).
+
+  (** ** Duplicable observation describing the prefix of a log. *)
+  Definition own_log_obs (γ : gname) (l : list A) : iProp Σ :=
+    own γ (◯ML l).
+
+  Lemma get_obs (γ : gname) (q : Qp) (l : list A) :
+    own_log_auth γ q l ⊢ own_log_obs γ l.
+  Proof.
+   iIntros "Hown".
+   rewrite /own_log_obs.
+   iApply (own_mono with "Hown").
+   apply mono_list_included.
+  Qed.
+
+  Lemma own_obs_prefix (γ : gname) (q : Qp) (L l : list A) :
+    own_log_auth γ q L ⊢ own_log_obs γ l -∗ ⌜l `prefix_of` L⌝.
+  Proof.
+   iIntros "Hown Hobs".
+   rewrite /own_log_obs.
+   iDestruct (own_valid_2 with "[$Hown][$Hobs]") as "%Hvalid".
+   apply mono_list_both_dfrac_valid_L in Hvalid.
+   naive_solver.
+  Qed.
+
+End Log_Resources_definition.
